KLR/NKI/Typed.lean
@@ -14,10 +14,8 @@ See the License for the specific language governing permissions and
 limitations under the License.
 -/
 
-import KLR.NKI.Annotations
-import KLR.NKI.Basic
-import KLR.NKI.Patterns
-import KLR.NKI.Pretty
-import KLR.NKI.Simplify
-import KLR.NKI.SimplifyOperators
-import KLR.NKI.Typed
+import KLR.NKI.Typed.Basic
+import KLR.NKI.Typed.Context
+import KLR.NKI.Typed.Elab
+import KLR.NKI.Typed.Test
+import KLR.NKI.Typed.Types
