KLR/NKI/Typed/Elab.lean
@@ -1,0 +1,1004 @@
+/-
+Copyright KLR Contributors
+
+Licensed under the Apache License, Version 2.0 (the "License");
+you may not use this file except in compliance with the License.
+You may obtain a copy of the License at
+
+     https://www.apache.org/licenses/LICENSE-2.0
+
+Unless required by applicable law or agreed to in writing, software
+distributed under the License is distributed on an "AS IS" BASIS,
+WITHOUT WARRANTIES OR CONDITIONS OF ANY KIND, either express or implied.
+See the License for the specific language governing permissions and
+limitations under the License.
+-/
+
+import KLR.NKI.Typed.Basic
+import KLR.NKI.Typed.Context
+import KLR.NKI.Typed.Types
+import KLR.Py.Pretty
+
+theorem List.ne_nil_of_not_empty {α} {l : List α} : ¬l.isEmpty = true → l ≠ [] := by
+  intro; simp_all only [isEmpty_iff, ne_eq, not_false_eq_true]
+
+namespace KLR.NKI.Typed
+
+open Py (Ident FileInfo Span)
+
+/-!
+# Elaboration that turns python into fully-typed NKI
+This implements the bidirectional typechecking algorithm described here:
+https://arxiv.org/abs/1306.6032
+
+Missing features:
+- Kind validation.
+  We currently run kind checking after inferring the type of a function def.
+  However, we pass it a empty kind context when doing so, this fails when
+  a nested `def` refers to a type variable bound earlier.
+  We should also think about whether `dtype` should be a separate kind.
+- Unimplemented language features, grep for calls of `throwUnsupported`
+- Semantic subtyping.
+  For example, if a function expects: `∀ DT M N, tensor[DT, (M, N, M + N)]`,
+  passing it `tensor[int, (10, 20, 30)]` should be allowed.
+- Better handling of subtyping coercions.
+  See comments in `Context.solve` and `stmt'` in the `ret` case.
+- Better error reporting in general.
+- Other todos marked by `TODO` comments.
+-/
+
+/-! # -----------Start: Parsing Type Annotations-------------- -/
+
+def prim : Py.Prim → Prim
+  | .none => .none
+  | .bool => .bool
+  | .numeric .int => .numeric .int
+  | .numeric .float => .numeric .float
+  | .string => .string
+  | .dtype dt => .dtype dt
+
+mutual
+
+def typ' (span : Span) (t : Py.Typ') : Typ :=
+  match t with
+  | .var id => .var span id
+  | .forall names body => .forall span (names.map (⟨·, []⟩)) (typ body)
+  | .prim p => .prim span (prim p)
+  | .func params ret => .func span (params.map typ) (typ ret)
+  | .size n => .size span n
+  | .shape dims => .shape span (dims.map typ)
+  | .tuple typs => .tuple span (typs.map typ)
+  | .list t => .list span (typ t)
+  | .tensor sh dt => .tensor span (typ sh) (typ dt)
+  | .iter t => .iter span (typ t )
+  | .sizeAdd x y => .sizeAdd span (typ x) (typ y)
+  | .shapeAppend s1 s2 => .shapeAppend span (typ s1) (typ s2)
+
+def typ : Py.Typ → Typ
+  | { span, typ := t } => typ' span t
+
+end
+
+/-! # -----------End: Parsing Type Annotations-------------- -/
+
+
+/-! # -----------Start: Type Checking Utilities -------------- -/
+
+abbrev KindCtx := Array (Array (Ident × Kind))
+
+def KindCtx.pop (Φ : KindCtx) : KindCtx := Array.pop Φ
+
+def KindCtx.push (Φ : KindCtx) (names : List Ident) : KindCtx :=
+  Array.push Φ (names.toArray.map fun name => (name, .unknown))
+
+def KindCtx.get? (Φ : KindCtx) (name : Ident) : Option Kind := do
+  for i in (List.finRange Φ.size).reverse do
+    let Γ := Φ[i]
+    for j in (List.finRange Γ.size).reverse do
+      let (name', kind) := Γ[j]
+      if name' == name then
+        return kind
+  none
+
+def KindCtx.update (Φ : KindCtx) (name : Ident) (kind : Kind) : KindCtx := Id.run do
+  let mut Φ := Φ
+  for i in (List.finRange Φ.size).reverse do
+    let Γ := Φ[i]
+    for j in (List.finRange Γ.size).reverse do
+      let (name', _) := Γ[j]
+      if name' == name then
+        let Γ := Γ.set j (name, kind)
+        return Φ.set i Γ
+  return Φ
+
+/--
+Check if a type is kind correct.
+NOTE: where bounds are ignored
+-/
+def Typ.checkKind (expected : Kind) (Φ : KindCtx) : Typ → ElabM KindCtx
+  | .var span id | .evar span id => withSpan span do
+    match Φ.get? id with
+    | some k =>
+      if k == .unknown then
+        return Φ.update id expected
+      else
+        if k == expected then
+          return Φ
+        else
+          throwType s!"kind mismatch, expected {expected}, got {k}"
+    | none => throwType "unbound type variable"
+  | .forall span vars body => do
+    if expected != .typ then withSpan span (throwType s!"kind mismatch, expected {expected}, got type") else
+    let Ψ ← body.checkKind .typ (Φ.push (vars.map TypVar.name))
+    return Ψ.pop
+  | .prim span _ =>
+    if expected == .typ then
+      return Φ
+    else
+      withSpan span (throwType s!"kind mismatch, expected {expected}, got type")
+  | .func span params ret => do
+    if expected != .typ then withSpan span (throwType s!"kind mismatch, expected {expected}, got type") else
+    let Φ ← params.foldlM (Typ.checkKind .typ) Φ
+    ret.checkKind .typ Φ
+  | .size span _ =>
+    if expected == .size then
+      return Φ
+    else
+      withSpan span (throwType s!"kind mismatch, expected {expected}, got size")
+  | .shape span dims =>
+    if expected != .shape then withSpan span (throwType s!"kind mismatch, expected {expected}, got shape. Did you mixed up the order of tensor shape and dtype?") else
+    dims.foldlM (Typ.checkKind .size) Φ
+  | .tuple span typs =>
+    if expected != .typ then withSpan span (throwType s!"kind mismatch, expected {expected}, got type") else
+    typs.foldlM (Typ.checkKind .typ) Φ
+  | .list span t =>
+    if expected != .typ then withSpan span (throwType s!"kind mismatch, expected {expected}, got type") else
+    t.checkKind .typ Φ
+  | .tensor span sh dt => do
+    if expected != .typ then withSpan span (throwType s!"kind mismatch, expected {expected}, got type") else
+    let Φ ← sh.checkKind .shape Φ
+    /- TODO: do we want to enforce a special kind for dtypes? -/
+    dt.checkKind .typ Φ
+  | .iter span t => do
+    if expected != .typ then withSpan span (throwType s!"kind mismatch, expected {expected}, got type") else
+    t.checkKind .typ Φ
+  | .sizeAdd span x y => do
+    if expected != .size then withSpan span (throwType s!"kind mismatch, expected {expected}, got size") else
+    let Φ ← x.checkKind .size Φ
+    y.checkKind .size Φ
+  | .shapeAppend span s1 s2 => do
+    if expected != .shape then withSpan span (throwType s!"kind mismatch, expected {expected}, got shape") else
+    let Φ ← s1.checkKind .shape Φ
+    s2.checkKind .shape Φ
+
+partial def Context.typewf (Γ : Context) (typ : Typ) : ElabM Unit := do
+  match typ with
+  | .var _ name =>
+    if !Γ.foralls.contains name then
+      throwType s!"type variable {name} not found in context"
+  | .evar _ name =>
+    if !Γ.existentials.contains name then
+      throwType s!"meta variable {name} not found in context"
+  | .forall _ vars body =>
+    let c' := Γ ++ (vars.map fun ⟨x, _⟩ => .forall x).toArray
+    c'.typewf body
+  | .func _ params ret =>
+    (Γ.typewf ret)
+    params.forM Γ.typewf
+  | .prim _ _
+  | .size _ _ => return
+  | .shape _ dims => dims.forM Γ.typewf
+  | .tuple _ typs => typs.forM Γ.typewf
+  | .list _ t => Γ.typewf t
+  | .tensor _ sh dt => Γ.typewf sh; Γ.typewf dt
+  | .iter _ t => Γ.typewf t
+  | .sizeAdd _ x y => Γ.typewf x; Γ.typewf y
+  | .shapeAppend _ s1 s2 => Γ.typewf s1; Γ.typewf s2
+
+def Context.solve (Γ : Context) (α : Ident) (t : Typ) : ElabM (Option Context) := do
+  Γ.typewf t
+  if !t.isMonotype then return none else
+  let some (cL, cR) := Γ.breakMarker (.exists α) | {
+    /-
+    If the code reaches here, it means we cannot find `.exists α` in the context,
+    implying that `α` is already solved since we replace `.exists α` with `.existsSolved α τ`
+    when solving types.
+
+    Normally, we would just return the existing context.
+    But in our system, we want things like `0 if True else 1.1` to be typed as `float`.
+    However, because we process the input from left-to-right, the type varialbe in the
+    polymorphic if-then-else operator will get assigned to `int` first.
+    So we need to see if `α` has been assigned to a subtype of `t` and upgrade them.
+
+    There might be a better way to do this.
+    -/
+    match t with
+    | .prim _ (.numeric .float) => return Γ.upgradeToFloat α
+    | _ => return Γ
+  }
+  return (cL ++ [ContextElem.existsSolved α t] ++ cR)
+
+mutual
+
+partial def instantiateL (Γ : Context) (span : Span) (α : Ident) (rhs : Typ) : ElabM Context := withSpan span do
+  Γ.typewf (.evar span α)
+  Γ.typewf rhs
+  match ← Γ.solve α rhs with
+  | some c => return c
+  | none =>
+    match rhs with
+    | .evar _ β =>
+      if Γ.ordered α β then
+        let some Γ ← Γ.solve β (.evar span α) | throwType s!"cannot substitute {rhs}"
+        return Γ
+      else
+        let some Γ ← Γ.solve α rhs | throwType s!"cannot substitute {rhs}"
+        return Γ
+    | .func _ params ret =>
+      let params' ← params.mapM fun _ => freshName
+      let ret' ← freshName
+      let α' := Typ.func span (params'.map (.evar span)) (.evar span ret')
+      let Θ : Context :=
+        #[ContextElem.exists ret'] ++ (params'.reverse.map ContextElem.exists) ++ #[.existsSolved α α']
+      let some Θ := Γ.insertAt (.exists α) Θ | throwType s!"failed to update context"
+      let Θ ← (params.zip params').foldlM (fun Γ (p, p') => instantiateR Γ p.span (Γ.apply p) p') Θ
+      instantiateL Θ ret.span ret' (Θ.apply ret)
+    | .forall _ vars body =>
+      let namePairs ← vars.mapM fun {name, ..} => return (name, ← freshName)
+      let Γ := Γ ++ namePairs.map fun (_, name) => ContextElem.forall name
+      let Θ ← instantiateL Γ body.span α (body.applySubsts (namePairs.map fun (name, name') => (name, .var span name')))
+      /- TODO: optimize this -/
+      return namePairs.foldl (fun Θ (_, β') => Θ.dropMarker (.forall β')) Θ
+    | _ => throwType s!"subtituting this polytype {rhs} not supported"
+
+partial def instantiateR (Γ : Context) (span : Span) (lhs : Typ) (α : Ident) : ElabM Context := withSpan span do
+  Γ.typewf lhs
+  Γ.typewf (.evar span α)
+  match ← Γ.solve α lhs with
+  | some c => return c
+  | none =>
+    match lhs with
+    | .evar _ β =>
+      if Γ.ordered α β then
+        let some Γ ← Γ.solve β (.evar span α) | throwType s!"cannot subtitute {lhs}"
+        return Γ
+      else
+        let some Γ ← Γ.solve α lhs | throwType s!"cannot substitute {lhs}"
+        return Γ
+    | .func _ params ret =>
+      let params' ← params.mapM fun _ => freshName
+      let ret' ← freshName
+      let α' := Typ.func span (params'.map (.evar span)) (.evar span ret')
+      let Θ : Context :=
+        #[ContextElem.exists ret'] ++ (params'.reverse.map ContextElem.exists) ++ #[.existsSolved α α']
+      let some Θ := Γ.insertAt (.exists α) Θ | throwType s!"failed to update context"
+      let Θ ← (params.zip params').foldlM (fun Γ (p, p') => instantiateL Γ p.span p' (Γ.apply p)) Θ
+      instantiateR Θ ret.span (Θ.apply ret) ret'
+    | .forall _ vars body =>
+      let namePairs ← vars.mapM fun {name, ..} => return (name, ← freshName)
+      let Γ := namePairs.foldl (fun Γ (_, β') => Γ ++ #[.marker β', .exists β']) Γ
+      let Θ ← instantiateR Γ body.span (body.applySubsts (namePairs.map fun (name, name') => (name, .evar span name'))) α
+      /- TODO: optimize this -/
+      return namePairs.foldl (fun Θ (_, β') => Θ.dropMarker (.marker β')) Θ
+    | _ => throwType s!"substituting this polytype {lhs} is not supported"
+
+end
+
+/-- Check if `lhs` is a subtype of `rhs`. -/
+partial def subtype (Γ : Context) (lhs rhs : Typ) : ElabM Context := do
+  Γ.typewf lhs
+  Γ.typewf rhs
+  match lhs, rhs with
+  | .var _ x, .var span y =>
+    if x == y then return Γ else
+    withSpan span (throwType s!"{y} does not match {x}")
+  | .evar span x, .evar _ y =>
+    let occurs := Γ.existentials.contains x
+    if x == y && occurs then return Γ else
+    if occurs then
+      instantiateL Γ span x rhs
+    else
+      withSpan span (throwType s!"{x} is not bound in the type context")
+  | .evar span x, rhs =>
+    if Γ.existentials.contains x && !rhs.ftv.contains x then
+      instantiateL Γ span x rhs
+    else
+      withSpan span (throwType s!"substitution of {x} is invalid")
+  | lhs, .evar span y =>
+    if Γ.existentials.contains y && !lhs.ftv.contains y then
+      instantiateR Γ span lhs y
+    else
+      withSpan span (throwType s!"substitution of {y} is invalid")
+  | lhs, .forall span vars body =>
+    let namePairs ← vars.mapM fun {name, ..} => return (name, ← freshName)
+    let substs : Substitutions := namePairs.map fun (name, name') => (name, .var span name')
+    let body := body.applySubsts substs
+    let fvars := namePairs.map fun (_, name) => ContextElem.forall name
+    let c' ← subtype (Γ ++ fvars) lhs body
+    /- TODO: optimize this -/
+    return fvars.foldl (fun c fv => c.dropMarker fv) c'
+  | .forall span vars body, rhs =>
+    let namePairs ← vars.mapM fun {name, ..} => return (name, ← freshName)
+    let substs : Substitutions := namePairs.map fun (name, name') => (name, .evar span name')
+    let body := body.applySubsts substs
+    let c' := namePairs.foldl (fun c (_, name) => c ++ #[(.marker name), (.exists name)]) Γ
+    let c' ← subtype c' body rhs
+    /- TODO: optimize this -/
+    return namePairs.foldl (fun c (_, ev) => c.dropMarker (.marker ev)) c'
+  | .prim span p1, .prim _ p2 => do
+    if (p1 == .numeric .int && p2 == .numeric .float) || p1 == p2 then
+      return Γ
+    else
+      withSpan span (throwType s!"expected {p2}, got {p1}")
+  | .func span paramsLhs retLhs, .func _ paramsRhs retRhs =>
+    let lhsLen := paramsLhs.length
+    let rhsLen := paramsRhs.length
+    if lhsLen ≠ rhsLen then withSpan span (throwType s!"wrong number of arguments, got {lhsLen} but expected {rhsLen}") else
+    let c ← (paramsLhs.zip paramsRhs).foldlM (fun c (lhs, rhs) => subtype c (c.apply rhs) (c.apply lhs)) Γ
+    subtype c retLhs retRhs
+  | .size span n, .size _ m => do
+    if n != m then
+      withSpan span (throwType s!"expected size to be {m}, got {n}")
+    else
+      return Γ
+  | .shape span lhs, .shape _ rhs =>
+    let lhsLen := lhs.length
+    let rhsLen := rhs.length
+    if lhsLen ≠ rhsLen then
+      withSpan span (throwType s!"tensor rank mismatch, expected rank {rhsLen}, got rank {lhsLen}")
+    else
+      (lhs.zip rhs).foldlM (fun c (lhs, rhs) => subtype c (c.apply lhs) (c.apply rhs)) Γ
+  | .tuple span lhs, .tuple _ rhs =>
+    let lhsLen := lhs.length
+    let rhsLen := rhs.length
+    if lhsLen ≠ rhsLen then
+      withSpan span (throwType s!"tuple length mismatch, expected length {rhsLen}, got length {lhsLen}")
+    else
+      (lhs.zip rhs).foldlM (fun c (lhs, rhs) => subtype c (c.apply lhs) (c.apply rhs)) Γ
+  | .list _ lhs, .list _ rhs => subtype Γ lhs rhs
+  | .tensor _ sh1 dt1, .tensor _ sh2 dt2 =>
+    let c ← subtype Γ sh1 sh2
+    subtype c dt1 dt2
+  | .iter _ lhs, .iter _ rhs => subtype Γ lhs rhs
+  | .sizeAdd span _ _, _
+  | _, .sizeAdd span _ _ => withSpan span (throwUnsupported "adding sizes")
+  | .shapeAppend span _ _, _
+  | _, .shapeAppend span _ _ => withSpan span (throwUnsupported "appending shapes")
+  | lhs, rhs => withSpan lhs.span (throwType s!"{lhs} is not a subtype of {rhs}")
+
+/-! # -----------End: Type Checking Utilities -------------- -/
+
+
+
+/-! # -----------Start: Elaborating Python to NKI -------------- -/
+
+def value : Py.Value → ElabM Value
+  | .none     => return .none
+  | .bool   v => return .bool   v
+  | .int    v => return .int    v
+  | .float  v => return .float  v
+  | .string v => return .string v
+  | .ellipsis => throwType "ellipsis only allowed in tensor index"
+
+def nonNumericBinOp : Py.BinOp → ElabM Builtin
+  | .land       => return .land
+  | .lor        => return .lor
+  | .ne         => return .ne
+  | .eq         => return .eq
+  | .rshift     => return .rshift
+  | .lshift     => return .lshift
+  | .bitwiseAnd => return .bitwiseAnd
+  | .bitwiseXor => return .bitwiseXor
+  | .bitwiseOr  => return .bitwiseOr
+  | .matmul     => return .matmul
+  | _           => throwInternal "nonNumericBinOp should not be called on this operator"
+
+def numericBinOp (n : Numeric) : Py.BinOp → ElabM Builtin
+  | .floor => return .floor n
+  | .pow   => return .pow n
+  | .mod   => return .mod n
+  | .div   => return .div n
+  | .mul   => return .mul n
+  | .sub   => return .sub n
+  | .add   => return .add n
+  | .ge    => return .ge n
+  | .gt    => return .gt n
+  | .le    => return .le n
+  | .lt    => return .lt n
+  | _      => throwInternal "numericBinOp should not be called on this operator"
+
+partial def applyTypArgs (args : List Typ) : Typ → ElabM (List Typ × Typ)
+  | .forall span vars body => do
+    let αs := vars.map TypVar.name
+    if args.length < αs.length then withSpan span (throwType "incorrect number of type arguments") else
+    let polies := args.filter (not ∘ Typ.isMonotype)
+    if let some poly := polies.head? then withSpan poly.span (throwType s!"cannot substitute a polymorphic type: {poly}") else
+    let subs : Substitutions := (αs.zip args).reverse
+    let body := body.applySubsts subs
+    applyTypArgs (args.drop αs.length) body
+  | .func span params ret =>
+    if h : args.length > 0 then withSpan args[0].span (throwType s!"unexpected type argument {args[0]}") else
+    return (params, ret)
+  | t => withSpan t.span (throwType s!"got type {t}, expected function type")
+
+partial def inferTypArgs (Γ : Context) (arrTyp : Typ) (numArgs : Nat) (typArgs : List Typ := []) : ElabM (List Typ × List Typ × Typ × Context) := do
+  Γ.typewf arrTyp
+  match arrTyp with
+  | .forall span vars body =>
+    let αs := vars.map TypVar.name
+    let αs' ← αs.mapM fun _ => freshName
+    let Θ := Γ ++ (αs'.map ContextElem.exists)
+    let subs : Substitutions := (αs.zip (αs'.map (.evar span))).reverse
+    let body := body.applySubsts subs
+    inferTypArgs Θ body numArgs (typArgs ++ (αs'.map (.evar span)))
+  | .evar span α =>
+    let params ← (List.range numArgs).mapM fun _ => freshName
+    let ret ← freshName
+    let paramTyps := params.map (Typ.evar span)
+    let retTyp := Typ.evar span ret
+    let Θ : Context := #[.exists ret] ++ (params.reverse.toArray.map .exists) ++ #[.existsSolved α (.func span paramTyps retTyp)]
+    let some Θ := Γ.insertAt (.exists α) Θ | throwType s!"failed to update context at {α}"
+    return (typArgs, paramTyps, retTyp, Θ)
+  | .func _ params ret =>
+    return (typArgs, params, ret, Γ)
+  | t => withSpan t.span (throwType s!"expected function type, got {t}")
+
+mutual
+
+partial def args (Γ : Context) : List Py.Arg → List Typ → ElabM (List Exp × List Typ × Context)
+  | [], [] => return ([], [], Γ)
+  | { keyword, val } :: aTl, tHd :: tTl => do
+    if keyword.isSome then throwUnsupported "keyword arguments" else
+    let (val, t, Γ) ← exp val Γ tHd
+    let (aTl, tTl, Γ) ← args Γ aTl tTl
+    return (val :: aTl, t :: tTl, Γ)
+  | hd :: _, [] => withSpan hd.val.span (throwType "unexpected extra argument")
+  | [], hd :: _ => throwType s!"missing argument of type {hd}"
+
+partial def expList (es : List Py.Exp) (ts : List (Option Typ)) (Γ : Context) : ElabM (List Exp × List Typ × Context) := do
+  match es, ts with
+  | [], [] => return ([], [], Γ)
+  | eHd :: eTl, tHd :: tTl =>
+    let (eHd, tHd, Γ) ← exp eHd Γ tHd
+    let (eTl, tTl, Γ) ← expList eTl tTl Γ
+    return (eHd :: eTl, tHd :: tTl, Γ)
+  | hd :: _, [] => withSpan hd.span (throwType s!"too many expressions")
+  | [], _ :: _ => throwType s!"missing expressions"
+
+/-- NOTE: We don't check for subsumption of the expected result type here, that's checked by `exp'` -/
+partial def mkApp (f : Exp) (arrTyp : Typ) (typArgs : List Py.Typ) (as : List Py.Arg) (Γ : Context) : ElabM (Exp × Typ × Context) := do
+  let typArgs := typArgs.map typ
+  let (typArgs, params, ret, Γ) ←
+    if !typArgs.isEmpty then
+      let (params, ret) ← applyTypArgs typArgs arrTyp
+      pure (typArgs, params, ret, Γ)
+    else
+      inferTypArgs Γ arrTyp as.length
+  let (as, _, Γ) ← args Γ as params
+  let typArgs := Γ.apply <$> typArgs
+  let ret := Γ.apply ret
+  return (.call (← getSpan!) f typArgs as, ret, Γ)
+
+partial def exp' (e : Py.Exp') (Γ : Context) (expected : Option Typ := none) : ElabM (Exp × Typ × Context) := do
+  let span ← getSpan!
+  let (e, typ, Γ) ←
+    match e with
+    | .var name =>
+      -- TODO: lookup a list of builtin functions here
+      let some found := Γ.findVarType name | throwType s!"variable not in scope"
+      let e := .var span name
+      pure (e, found, Γ)
+    | .value v =>
+      let v ← value v
+      let e := Exp.value span v
+      let checked := v.typ span
+      pure (e, checked, Γ)
+    | .unaryOp op x => do
+      match op with
+      | .pos =>
+        let (x, xTyp, Γ) ← exp x Γ
+        let Γ ← subtype Γ xTyp (floatTyp span)
+        pure (x, Γ.apply xTyp, Γ)
+      | .neg =>
+        let (x, xTyp, Γ) ← exp x Γ
+        let Γ ← subtype Γ xTyp (floatTyp span)
+        let xTyp := Γ.apply xTyp
+        let op ←
+          match xTyp with
+          | .prim _ (.numeric .int) => pure (Builtin.neg .int)
+          | .prim _ (.numeric .float) => pure (Builtin.neg .float)
+          | _ => throwType s!"type mismatch, got {xTyp}, expected int or float"
+        pure (.call span (.builtin span op) [] [x], xTyp, Γ)
+      | .bitwiseNot =>
+        let (x, xTyp, Γ) ← exp x Γ (intTyp span)
+        pure (.call span (.builtin span .bitwiseNot) [] [x], xTyp, Γ)
+      | .lnot =>
+        let (x, xTyp, Γ) ← exp x Γ (boolTyp span)
+        pure (.call span (.builtin span .lnot) [] [x], xTyp, Γ)
+    | .binOp op x y => do
+      match op with
+      -- -- logical
+      | .land | .lor =>
+        let (x, _, Γ) ← exp x Γ (boolTyp x.span)
+        let (y, _, Γ) ← exp y Γ (boolTyp y.span)
+        let op ← nonNumericBinOp op
+        pure (.call span (.builtin span op) [] [x, y], boolTyp span, Γ)
+      -- bitwise
+      | .bitwiseOr | .bitwiseXor | .bitwiseAnd
+      | .lshift | .rshift =>
+        let (x, _, Γ) ← exp x Γ (intTyp x.span)
+        let (y, _, Γ) ← exp y Γ (intTyp y.span)
+        let op ← nonNumericBinOp op
+        pure (.call span (.builtin span op) [] [x, y], intTyp span, Γ)
+      -- comparison
+      | .eq | .ne =>
+        let op ← nonNumericBinOp op
+        let arrTyp := op.typ span
+        mkApp (.builtin span op) arrTyp [] [{val := x}, {val := y}] Γ
+      -- arithmetic comparison
+      | .lt | .le | .gt | .ge =>
+        let (x, xTyp, Γ) ← exp x Γ
+        let (y, yTyp, Γ) ← exp y Γ
+        let Γ ← subtype Γ xTyp (floatTyp span)
+        let Γ ← subtype Γ (Γ.apply yTyp) (floatTyp span)
+        let yTyp := Γ.apply yTyp
+        let n : Numeric :=
+          match xTyp, yTyp with
+          | .prim _ (.numeric .float), _
+          | _, .prim _ (.numeric .float) => .float
+          | _, _ => .int
+        let op ← numericBinOp n op
+        pure (.call span (.builtin span op) [] [x, y], boolTyp span, Γ)
+      -- arithmetic
+      | .add | .sub | .mul | .div
+      | .mod | .pow | .floor =>
+        let (x, xTyp, Γ) ← exp x Γ
+        let (y, yTyp, Γ) ← exp y Γ
+        let Γ ← subtype Γ xTyp (floatTyp span)
+        let Γ ← subtype Γ (Γ.apply yTyp) (floatTyp span)
+        let yTyp := Γ.apply yTyp
+        let n : Numeric :=
+          match xTyp, yTyp with
+          | .prim _ (.numeric .float), _
+          | _, .prim _ (.numeric .float) => .float
+          | _, _ => .int
+        let op ← numericBinOp n op
+        pure (.call span (.builtin span op) [] [x, y], numericTyp span n, Γ)
+      | .matmul => throwUnsupported "matmul"
+    | .tuple es => do
+      let expectedTyps : List (Option Typ) ←
+        match expected with
+        | none => pure (List.replicate es.length none)
+        | some (.tuple span expected) =>
+          if expected.length ≠ es.length then
+            withSpan span (throwType s!"expected tuple with {expected.length} elements, got one with {es.length} elements")
+          else
+            pure (expected.map some)
+        | some t => withSpan t.span (throwType s!"expected tuple, got {t}")
+      let (es, ts, Γ) ← expList es expectedTyps Γ
+      pure (.tuple span es, .tuple span ts, Γ)
+    | .list es => do
+      let expectedTyps : List (Option Typ) ←
+        match expected with
+        | none => pure (List.replicate es.length none)
+        | some (.list _ t) => pure (List.replicate es.length (some t))
+        | some t => withSpan t.span (throwType s!"expected list type, got {t}")
+      let (es, ts, Γ) ← expList es expectedTyps Γ
+      let α ← freshName
+      let Γ := Γ.push (.exists α)
+      let Γ ← ts.foldlM (fun Γ t => subtype Γ (.evar span α) (Γ.apply t)) Γ
+      pure (.list span es, .list span (Γ.apply (.evar span α)), Γ)
+    | .ifExp test body orelse => do
+      let f : Exp := .builtin span .ite
+      let arrTyp := Builtin.ite.typ span
+      mkApp f arrTyp [] [{val := test}, {val := body}, {val := orelse}] Γ
+    | .call f typArgs as => do
+      let (f, arrTyp, Γ) ← exp f Γ
+      mkApp f arrTyp typArgs as Γ
+    | .access _ _ =>
+      throwUnsupported "subscript expression"
+    | .attr _ _ =>
+      throwUnsupported "attribute access"
+  match expected with
+  | some expected =>
+    let Γ ← subtype Γ typ expected
+    return (e, Γ.apply typ, Γ)
+  | none => return (e, typ, Γ)
+
+partial def exp (e : Py.Exp) (Γ : Context) (expected : Option Typ := none) : ElabM (Exp × Typ × Context) :=
+  match e with
+  | { span, exp } => withSpan span do exp' exp Γ expected
+
+end
+
+/--
+NOTE: No correctness check is done
+-/
+partial def Typ.applyArr (arr : Typ) (typArgs : List Typ) (args : List Typ) : Option Typ :=
+  match arr with
+  | .forall _ vars body =>
+    if vars.length > typArgs.length then none else
+    let names := vars.map TypVar.name
+    let subs : Substitutions := (names.zip typArgs).reverse
+    let body := body.applySubsts subs
+    body.applyArr (typArgs.drop names.length) args
+  | .func _ params ret =>
+    if args.length > params.length then none else
+    if args.length = params.length then ret else
+    ret.applyArr [] (args.drop params.length)
+  | _ => none
+
+def Exp.typ (e : Exp) (Γ : Context) : ElabM Typ :=
+  match e with
+  | .var _ id => do
+    let some t := Γ.findVarType id | throwType s!"variable {id} cannot be found in the context"
+    return t
+  | .value span val => return val.typ span
+  | .builtin span val => return val.typ span
+  | .tuple span es => (.tuple span ·) <$> (es.mapM (Exp.typ · Γ))
+  | .list span es => do
+    let es ← es.mapM (Exp.typ · Γ)
+    (Typ.list span ·) <$> es.head?
+  | .call _ f typArgs args => do
+    let arrT ← f.typ Γ
+    let argsT ← args.mapM (Exp.typ · Γ)
+    arrT.applyArr typArgs argsT
+
+/--
+`desired` is the type the user wants, used to "admit" a definition using `pass`
+-/
+def Stmt.typ (s : Stmt) (Γ : Context) (desired : Typ) : ElabM Typ :=
+  match s with
+  | .seq _ _ s2 => s2.typ Γ desired
+  | .exp span _ => return noneTyp span
+  | .ret _ e => e.typ Γ
+  | .letBind _ name typ _ body =>
+    /-
+    NOTE: we have to re-introduce the variable in the context because it is
+    dropped after the let-assignment statement has been elaborated.
+    -/
+    body.typ (Γ ++ #[.var name typ]) desired
+  | .assign span _ _ => return noneTyp span
+  | .assert span _ => return noneTyp span
+  | .funcDef _ _ t _ => return t
+  | .ifStm _ _ thn els =>
+    match els with
+    | some els => do
+      let t1 ← thn.typ Γ desired
+      let t2 ← els.typ Γ desired
+      return t1.min t2
+    | none => thn.typ Γ desired
+  | .forLoop span _ _ _ => return noneTyp span
+  | .whileLoop span _ _ => return noneTyp span
+  | .pass _ => return desired
+  | .breakLoop span => return noneTyp span
+  | .continueLoop span => return noneTyp span
+
+def Stmt.append (s1 : Stmt) : Option Stmt → Stmt
+  | some s2 => .seq ⟨s1.span.pos, s2.span.stopPos⟩ s1 s2
+  | none    => s1
+
+abbrev BoundsCtx := Array (Ident × (Kind × List TypBound))
+
+def BoundsCtx.get? (c : BoundsCtx) (name : Ident) : Option (Kind × List TypBound) := do
+  for i in (List.finRange c.size).reverse do
+    let (name', kbs) := c[i]
+    if name' == name then return kbs
+  none
+
+def BoundsCtx.set (c : BoundsCtx) (name : Ident) (kind : Kind) (bounds : List TypBound) : BoundsCtx := Id.run do
+  let mut c := c
+  for i in (List.finRange c.size).reverse do
+    let (name', _) := c[i]
+    if name' == name then return Array.set c i (name, (kind, bounds))
+  return c
+
+def whereBound (c : BoundsCtx) (e : Py.Exp) : ElabM BoundsCtx := do
+  match e with
+  | ⟨_, .binOp .bitwiseOr ⟨factorSpan, .value (.int factor)⟩ ⟨varSpan, .var t⟩⟩ =>
+    -- divisibility
+    -- `n | t` where `n` is a nat and `t` is a type var
+    if factor ≤ 0 then withSpan factorSpan (throwType "factor must be greater than 0") else
+    let some (kind, bounds) := c.get? t | withSpan varSpan (throwType "unbound type variable")
+    if kind != .size && kind != .unknown then withSpan varSpan (throwType s!"kind mismatch, expected size, got {kind}")
+    return c.set t .size (.divisibleBy factor.toNat :: bounds)
+  | ⟨_, .binOp .le ⟨varSpan, .var t⟩ ⟨upperSpan, .value (.int upper)⟩⟩ =>
+    -- less-than-equal-to
+    -- `t <= n` where `n` is a nat and `t` is a type var
+    if upper ≤ 0 then withSpan upperSpan (throwType "upper bound must be greater than 0") else
+    let some (kind, bounds) := c.get? t | withSpan varSpan (throwType "unbound type variable")
+    if kind != .size && kind != .unknown then withSpan varSpan (throwType s!"kind mismatch, expected size, got {kind}")
+    return c.set t .size (.le upper.toNat :: bounds)
+  | e => withSpan e.span (throwType "unsupported where bound")
+
+def Exp.checkWhereBounds (Γ : Context) (e : Exp) : ElabM Unit :=
+  visit e
+where
+  visitList
+  | [] => return
+  | hd :: tl => do visit hd; visitList tl
+
+  visit
+  | .var _ _ => return
+  | .value _ _ => return
+  | .builtin _ _ => return
+  | .tuple _ es => visitList es
+  | .list _ es => visitList es
+  | .call _ f typArgs args => do
+    match ← f.typ Γ with
+    | .forall span vars _ =>
+      if vars.length ≠ typArgs.length then withSpan span (throwType "number of generic parameters does not match") else
+      (vars.zip typArgs).forM fun (⟨_, bounds⟩, t) =>
+        match t with
+        | .size span n =>
+          bounds.forM fun bound => do
+            match bound with
+            | .le m =>
+              if n > m then
+                withSpan span (throwType s!"size here must be less-than-equal-to {m}")
+            | .divisibleBy m =>
+              if n % m ≠ 0 then
+                withSpan span (throwType s!"size here must be divisible by {m}")
+        | .var _ _ => /- our analysis is conservative -/ return
+        | t => do
+          if !bounds.isEmpty then
+            withSpan t.span (throwType "expected size here")
+      visitList args
+    | _ => return
+
+/--
+Check if where bounds are satisfied in type applications
+-/
+def Stmt.checkWhereBounds (Γ : Context) (s : Stmt) : ElabM Unit :=
+  visit s
+where
+  visit
+  | .seq _ s1 s2 => do visit s1; visit s2
+  | .exp _ e => e.checkWhereBounds Γ
+  | .ret _ e => e.checkWhereBounds Γ
+  | .letBind _ _ _ rhs body => do rhs.checkWhereBounds Γ; visit body
+  | .assign _ lhs rhs => do lhs.checkWhereBounds Γ; rhs.checkWhereBounds Γ
+  | .assert _ e => do e.checkWhereBounds Γ
+  | .funcDef _ _ _ body => do visit body
+  | .ifStm _ cond thn els => do
+    cond.checkWhereBounds Γ
+    visit thn
+    match els with
+    | some els => visit els
+    | none => return
+  | .forLoop _ _ it body => do it.checkWhereBounds Γ; visit body
+  | .whileLoop _ cond body => do cond.checkWhereBounds Γ; visit body
+  | .pass _ => return
+  | .breakLoop _ => return
+  | .continueLoop _ => return
+
+mutual
+
+def stmts? : Option (List Py.Stmt) → Context → ElabM (Option Stmt × Context)
+  | some s, Γ => do
+    let (some s, Γ) ← stmts s Γ | throwEmptyStmts
+    return (some s, Γ)
+  | none, Γ => return (none, Γ)
+termination_by s => sizeOf s
+
+def elseIfs (elifs : List (Py.Exp × List Py.Stmt)) (els : Option (List Py.Stmt)) (Γ : Context) : ElabM (Option Stmt × Context) := do
+  match elifs with
+  | [] => stmts? els Γ
+  | (cond, thn) :: tl =>
+    let span ← getSpan!
+    let (cond, _, Γ) ← exp cond Γ (boolTyp span)
+    let (some thn, Γ) ← stmts thn Γ | throwEmptyStmts
+    let (els, Γ) ← elseIfs tl els Γ
+    return (some (.ifStm span cond thn els), Γ)
+termination_by sizeOf elifs + sizeOf els
+
+def funcDef (func : Py.FuncDef) (Γ : Context) : ElabM (Stmt × Context) := do
+  match func with
+  | { name, typParams, params, returns, body, decorators, whereBounds } =>
+    if !decorators.isEmpty then throwUnsupported "decorators" else
+    let span ← getSpan!
+
+    /- Compute the context extension needed -/
+    let Θ : Context := typParams.toArray.map .forall
+    let (paramTyps, Θ) ← params.foldlM (fun (pts, Θ) { typ := t, name, dflt } => do
+      if Option.isSome dflt then throwUnsupported "default argument" else
+      match t with
+      | some t =>
+        let t := typ t
+        return (pts.push t, Θ.push (.var name t))
+      | none =>
+        let α ← freshName
+        let t := .evar span α
+        return (pts.push t, Θ ++ #[.exists α, .var name t])
+    ) (#[], Θ)
+
+    let (retTyp, Θ) ←
+      match returns with
+      | some returns => pure (typ returns, Θ)
+      | none =>
+        let α ← freshName
+        pure (.evar span α, Θ.push (.exists α))
+
+    let markerName ← freshName
+    let Γ : Context := Γ ++ #[.marker markerName] ++ Θ
+
+    let (some body, Γ) ← withRetTyp retTyp (stmts body Γ) | throwEmptyStmts
+
+    let retTyp := Γ.apply retTyp
+    /-
+    Need to double check here to make sure if-statements are typed properly
+    -/
+    let Γ ← subtype Γ (← body.typ Γ retTyp) retTyp
+    let retTyp := Γ.apply retTyp
+    let funTyp := Γ.apply (Typ.func span paramTyps.toList retTyp)
+
+    /-
+    Must do this after all type inference is complete
+
+    TODO: find a better place to call this function.
+    Currently, we are not checking top-level code outside function definitions.
+    We are also not checking for default parameters because we need the context
+    to include all the parameters declared for the function.
+    -/
+    _ ← body.checkWhereBounds Γ
+
+    let some (Γ, Γ') := Γ.breakMarker (.marker markerName) | throwInternal "marker not found in context"
+    let genArgs := (Γ'.unsolved)
+    let (typParams, typBody) :=
+      if genArgs.isEmpty then
+        if typParams.isEmpty then (#[], funTyp) else (typParams.toArray, funTyp)
+      else
+        /-
+        TODO: rename the inferred type parameters to be more user friendly.
+        Need to be careful about capture avoidance while doing so.
+        -/
+        let subs : Substitutions := genArgs.toList.map fun α => (α, .var span α)
+        let body := funTyp.applySubsts subs
+        ((genArgs ++ typParams.toArray), body)
+
+    /-
+    TODO:
+    First, we need to properly keep track of the kind of each type variable currently in bound.
+    Here, we always pass an empty context which is fine until we need to check the type of a nested
+    function definition.
+
+    Second, we need the kind of each top-level type variable for the whereBounds, this is a bit of a hack to get it.
+    -/
+    let kindCtx ← typBody.checkKind .typ (KindCtx.push #[] typParams.toList)
+    if h : kindCtx.size ≠ 1 then throwInternal "kind check returned the wrong number of scopes" else
+    let kindCtx := kindCtx[0]
+
+    let boundsCtx : BoundsCtx := kindCtx.map fun (name, kind) => (name, (kind, []))
+    let boundsCtx ← whereBounds.foldlM (fun c e => whereBound c e) boundsCtx
+
+    let typVars : List TypVar := boundsCtx.toList.map fun (id, (_, bounds)) => ⟨id, bounds⟩
+    let finalTyp :=
+      if typVars.isEmpty then typBody else .forall span typVars typBody
+
+    let fd := .funcDef span name finalTyp body
+    return (fd, Γ ++ #[.var name finalTyp])
+termination_by sizeOf func
+
+/--
+NOTE: Do not lift the call to `stmts k` up to the top of the function!
+This is becase some statements needs to modify the typing context before
+evaluating the continutation.
+-/
+def stmt' (s : Py.Stmt') (k : List Py.Stmt) (Γ : Context) : ElabM (Stmt × Context) := do
+  let span ← getSpan!
+  match s with
+  | .exp e =>
+    let (e, _, Γ) ← exp e Γ
+    let (k, Γ) ← stmts k Γ
+    return ((Stmt.exp span e).append k,  Γ)
+  | .imprt _ _ | .imprtFrom _ _ _ =>
+    throwUnsupported "import statements"
+  | .ret e =>
+    let (e, t, Γ) ← exp e Γ
+    let some retTyp ← getRetTyp | throwType "\'return\' not allowed outside function contexts"
+    /-
+    TODO: The way we check and update the return type here makes this valid program a type error:
+    ```
+    def ite():
+      if True:
+        return 0
+      else:
+        return 0.
+    ```
+    This function should have type `func[float]`, but we get a type error in the else branch
+    because the return type has already be set to `int`. We need to somehow carefully generalize
+    the return type here.
+    -/
+    let Γ ← subtype Γ t retTyp
+    applyCtxToRet Γ
+    let (k, Γ) ← stmts k Γ
+    return ((Stmt.ret span e).append k, Γ)
+  | .assign lhs anno rhs =>
+    let anno := anno.map typ
+    let (rhs, t, Γ) ← exp rhs Γ anno
+    match lhs with
+    | ⟨span, .var name⟩ =>
+      /- If name collisions were an issue, we would subtitute `name` in `rhs`
+         with a fresh variable. But our generated name never clashes with
+         user defined identifiers. So we simply make a marker here to know
+         which part of the output context to drop. -/
+      let α ← freshName
+      let Γ := Γ ++ #[.marker α, .var name t]
+      let (k, Γ) ← stmts k Γ
+      let k := k.getD (.exp span (.value span .none))
+      let some (Γ, _) := Γ.breakMarker (.marker α) | throwInternal "failed to find marker defined before"
+      /- Note that we do not generalize let-bindings as in other let-polymorphic type systems.
+         This decision can be revisited later. -/
+      return (Stmt.letBind span name t rhs k, Γ)
+    | _ => throwUnsupported "complex assignments"
+  | .assert e =>
+    let (e, t, Γ) ← exp e Γ
+    let Γ ← subtype Γ t (boolTyp span)
+    let (k, Γ) ← stmts k Γ
+    return ((Stmt.assert span e).append k, Γ)
+  | .funcDef dfn =>
+    let (dfn, Γ) ← funcDef dfn Γ
+    let (k, Γ) ← stmts k Γ
+    return (dfn.append k, Γ)
+  | .ifStm cond thn elifs els =>
+    let (cond, _, Γ) ← exp cond Γ (boolTyp span)
+    let (some thn, Γ) ← stmts thn Γ | throwEmptyStmts
+    let (els, Γ) ← elseIfs elifs els Γ
+    let (k, Γ) ← stmts k Γ
+    return ((Stmt.ifStm span cond thn els).append k, Γ)
+  | .forLoop pat iter body =>
+    match pat with
+    | .var name =>
+      let α ← freshName
+      let Γ := Γ ++ #[.marker α, .exists α, .var name (.evar span α)]
+      let (iter, _, Γ) ← exp iter Γ (Typ.iter span (.evar span α))
+      let (some body, Γ) ← withLoop (stmts body Γ) | throwEmptyStmts
+      let (k, Γ) ← stmts k Γ
+      let some (Γ, _) := Γ.breakMarker (.marker α) | throwInternal "cannot find marker in context"
+      return ((Stmt.forLoop span (.var name) iter body).append k, Γ)
+    | .tuple _ =>
+      throwUnsupported "tuple patterns"
+  | .whileLoop cond body =>
+    let (cond, _, Γ) ← exp cond Γ (boolTyp span)
+    let (some body, Γ) ← withLoop (stmts body Γ) | throwEmptyStmts
+    let (k, Γ) ← stmts k Γ
+    return ((Stmt.whileLoop span cond body).append k, Γ)
+  | .pass =>
+    let (k, Γ) ← stmts k Γ
+    return ((Stmt.pass span).append k, Γ)
+  | .breakLoop =>
+    if !(← inLoop) then throwType "\'break\' only allowed in loops" else
+    let (k, Γ) ← stmts k Γ
+    return ((Stmt.breakLoop span).append k, Γ)
+  | .continueLoop =>
+    if !(← inLoop) then throwType "\'continue\' only allowed in loops" else
+    let (k, Γ) ← stmts k Γ
+    return ((Stmt.continueLoop span).append k, Γ)
+termination_by sizeOf s + sizeOf k
+
+def stmt (s : Py.Stmt) (k : List Py.Stmt) (Γ : Context) : ElabM (Stmt × Context) := do
+  match s with
+  | { stmt, span } => withSpan span do stmt' stmt k Γ
+termination_by sizeOf s + sizeOf k
+
+def stmts (k : List Py.Stmt) (Γ : Context) : ElabM (Option Stmt × Context) := do
+  match k with
+  | [] => return (none, Γ)
+  | hd :: tl =>
+    let (s, Γ) ← stmt hd tl Γ
+    return (some s, Γ)
+termination_by sizeOf k
+
+end
+
+/-! # -----------End: Elaborating Python to NKI -------------- -/
+
+def typecheck (info : FileInfo) (p : Py.Prog) : Except String Context :=
+  match (stmts p.stmts #[]).run info {} with
+  | .ok (_, c) _ => .ok c
+  | .error msg _ => .error msg
+
+def runTypechecker (input : String) (fileName : String) (fileMap : Lean.FileMap := input.toFileMap) : Except String String := do
+  let prog ← Py.Parser.run input fileName fileMap
+  let c ← typecheck { content := input, fileName, fileMap } prog
+  return "\n".intercalate (c.toList.map ContextElem.toString)
